

Introduction to Linear Algebra (Gilbert Strang): 5th Ed.
Problem set 1.3)

Date _____

1) $3s_1 + 4s_2 + 5s_3 = b$.

$$\begin{bmatrix} 3 \\ 3 \\ 3 \end{bmatrix} + \begin{bmatrix} 0 \\ 4 \\ 4 \end{bmatrix} + \begin{bmatrix} 0 \\ 0 \\ 5 \end{bmatrix} = \begin{bmatrix} 3 \\ 7 \\ 12 \end{bmatrix} = b$$

$$\begin{bmatrix} 1 & 0 & 0 \\ 1 & 1 & 0 \\ 1 & 1 & 1 \end{bmatrix} \begin{bmatrix} 3 \\ 4 \\ 5 \end{bmatrix} = \begin{bmatrix} 3 \\ 7 \\ 12 \end{bmatrix}$$

2) $\begin{bmatrix} 1 & 0 & 0 \\ 1 & 1 & 0 \\ 1 & 1 & 1 \end{bmatrix} \begin{bmatrix} y_1 \\ y_2 \\ y_3 \end{bmatrix} = \begin{bmatrix} 1 \\ 1 \\ 1 \end{bmatrix}$, $y_1 = 1$
 $y_1 + y_2 = 1 \Rightarrow y_2 = 0$
 $y_1 + y_2 + y_3 = 1 \Rightarrow y_3 = 0$

$\begin{bmatrix} 1 & 0 & 0 \\ 1 & 1 & 0 \\ 1 & 1 & 1 \end{bmatrix} \begin{bmatrix} y_1 \\ y_2 \\ y_3 \end{bmatrix} = \begin{bmatrix} 1 \\ 4 \\ 9 \end{bmatrix}$, $y_1 = 1$
 $y_1 + y_2 = 4 \Rightarrow y_2 = 3$
 $y_1 + y_2 + y_3 = 9 \Rightarrow y_3 = 5$

4) $w_1 - 2w_2 + w_3 = 0$.

$$\begin{bmatrix} 1 \\ 3 \\ 3 \end{bmatrix} - 2 \begin{bmatrix} 4 \\ 0 \\ 0 \end{bmatrix} + \begin{bmatrix} 3 \\ 0 \\ 9 \end{bmatrix}$$

$$= \begin{bmatrix} 1 \\ 3 \\ 3 \end{bmatrix} - \begin{bmatrix} 8 \\ 0 \\ 0 \end{bmatrix} + \begin{bmatrix} 3 \\ 0 \\ 9 \end{bmatrix} = \begin{bmatrix} 0 \\ 0 \\ 0 \end{bmatrix}$$

They are on the same plane.

\therefore they are dependent

5) 1st set = $(y_1 = 1, y_2 = -2, y_3 = 1)$

2nd set = $(y_1 = 2, y_2 = -4, y_3 = 2)$

b) $\begin{bmatrix} 1 & 0 & 0 \\ 3 & 2 & 1 \\ 7 & 4 & c \end{bmatrix} \rightarrow c = 3$ $\begin{bmatrix} 1 \\ 3 \\ 7 \end{bmatrix} - \begin{bmatrix} 1 \\ 2 \\ 4 \end{bmatrix} - \begin{bmatrix} 0 \\ 0 \\ 0 \end{bmatrix} = \begin{bmatrix} 0 \\ 0 \\ 0 \end{bmatrix}$

$\begin{bmatrix} 1 & 0 & 0 \\ 1 & 1 & 0 \\ 0 & 1 & 1 \end{bmatrix} \rightarrow c = -1$ $-\begin{bmatrix} 1 \\ 1 \\ 0 \end{bmatrix} + \begin{bmatrix} 0 \\ 1 \\ 1 \end{bmatrix} - \begin{bmatrix} 0 \\ 0 \\ 0 \end{bmatrix} = \begin{bmatrix} 0 \\ 0 \\ 0 \end{bmatrix}$

$\begin{bmatrix} c & c & c \\ 2 & 1 & 7 \\ 3 & 3 & 6 \end{bmatrix} \rightarrow c = 0$ $\begin{bmatrix} 0 \\ 0 \\ 0 \end{bmatrix} - \begin{bmatrix} 0 \\ 1 \\ 3 \end{bmatrix} - \begin{bmatrix} 0 \\ 0 \\ 0 \end{bmatrix} = \begin{bmatrix} 0 \\ 0 \\ 0 \end{bmatrix}$

7) $a_1 \cdot a_1 + a_2 \cdot a_2 + a_3 \cdot a_3 = 0$.

Also, $r_1 \cdot r = 0$, $r_2 \cdot r = 0$, $r_3 \cdot r = 0$.

All three rows are perpendicular to r .

8) $\begin{bmatrix} 1 & 0 & 0 & 0 \\ -1 & 1 & 0 & 0 \\ 0 & -1 & 1 & 0 \\ 0 & 0 & -1 & 1 \end{bmatrix} \begin{bmatrix} x_1 \\ x_2 \\ x_3 \\ x_4 \end{bmatrix} = \begin{bmatrix} b_1 \\ b_2 \\ b_3 \\ b_4 \end{bmatrix}$

$x_1 = b_1$	$x_1 = b_1$
$-x_1 + x_2 = b_2$	$x_2 = b_1 + b_2$
$-x_2 + x_3 = b_3$	$x_3 = b_2 + b_3$
$-x_3 + x_4 = b_4$	$x_4 = b_3 + b_4$

$A^{-1} = \begin{bmatrix} 1 & 0 & 0 & 0 \\ 1 & 1 & 0 & 0 \\ 0 & 1 & 1 & 0 \\ 0 & 0 & 1 & 1 \end{bmatrix} \begin{bmatrix} b_1 \\ b_2 \\ b_3 \\ b_4 \end{bmatrix} = A^{-1}b$

9) $\begin{bmatrix} 1 & -0 & 0 & -1 \\ 0 & 1 & -1 & 0 \\ -1 & 0 & 1 & 0 \\ 0 & -1 & 0 & 1 \end{bmatrix} \begin{bmatrix} x_1 \\ x_2 \\ x_3 \\ x_4 \end{bmatrix} = \begin{bmatrix} 0 \\ 0 \\ 0 \\ 0 \end{bmatrix}$

$x_1 - x_4 = 0$

$x_2 - x_3 = 0$

$-x_1 + x_3 = 0$

$-x_2 + x_4 = 0 \Rightarrow \therefore x_1 = x_2 = x_3 = x_4$

\therefore when $d = \begin{bmatrix} c \\ c \\ c \\ c \end{bmatrix}$

Problem set 1.3)

$$10) \begin{bmatrix} z_2 - z_1 \\ z_3 - z_2 \\ 0 - z_3 \end{bmatrix} = \begin{bmatrix} b_1 \\ b_2 \\ b_3 \end{bmatrix}$$

$$\Delta^T \text{ in } z = \Delta^T b$$

$$= \begin{bmatrix} -1 & -1 & -1 \\ 0 & -1 & -1 \\ 0 & 0 & -1 \end{bmatrix} \begin{cases} z_2 - z_1 = b_1 \\ z_3 - z_2 = b_2 \\ 0 - z_3 = b_3 \end{cases}$$

$$z_3 = -b_3, z_2 = -b_2 - b_3, z_1 = -b_1 - b_2 - b_3$$

12) Invertible matrix C =

$$\begin{bmatrix} 0 & 1 & 0 & 0 \\ -1 & 0 & 1 & 0 \\ 0 & -1 & 0 & 1 \\ 0 & 0 & -1 & 0 \end{bmatrix} \begin{bmatrix} x_1 \\ x_2 \\ x_3 \\ x_4 \end{bmatrix} = \begin{bmatrix} x_2 \\ -x_1 + x_3 \\ -x_2 + x_4 \\ -x_3 \end{bmatrix} = \begin{bmatrix} b_1 \\ b_2 \\ b_3 \\ b_4 \end{bmatrix}$$

$$\begin{cases} x_2 = b_1 \\ x_3 = -b_4 \\ x_1 = -b_2 - b_4 \\ x_4 = b_1 + b_3 \end{cases} \rightarrow x = \begin{bmatrix} -b_2 - b_4 \\ b_1 \\ -b_4 \\ b_1 + b_3 \end{bmatrix}$$